theories/simplang/locations.v
@@ -4,7 +4,7 @@ From stdpp Require Import countable numbers gmap.
 (* partly adapted from lambda rust *)
 
 Definition block := positive.
-Record loc := { loc_chunk : block; loc_idx : Z }.
+Record loc := mkloc { loc_chunk : block; loc_idx : Z }.
 
 Global Instance loc_eq_decision : EqDecision loc.
 Proof. solve_decision. Qed.
@@ -29,15 +29,16 @@ Proof. destruct l; rewrite /loc_add /=; f_equal; lia. Qed.
 
 Lemma loc_add_0 l : l +ₗ 0 = l.
 Proof. destruct l; rewrite /loc_add /=; f_equal; lia. Qed.
+Lemma loc_add_block l n : loc_chunk (l +ₗ n) = loc_chunk l.
+Proof. done. Qed.
 
 Global Instance loc_add_inj l : Inj eq eq (loc_add l).
 Proof. destruct l; rewrite /Inj /loc_add /=; intros; simplify_eq; lia. Qed.
 
-Lemma loc_eta l : (Build_loc (loc_chunk l) (loc_idx l)) = l.
+Lemma loc_eta l : (mkloc (loc_chunk l) (loc_idx l)) = l.
 Proof.  by destruct l. Qed.
-Lemma Build_loc_add b i : Build_loc b 0 +ₗ i = Build_loc b i.
+Lemma mkloc_add b i : mkloc b 0 +ₗ i = mkloc b i.
 Proof. rewrite /loc_add; cbn. by replace (0 + i)%Z with i%Z by lia. Qed.
-
 Definition fresh_block {X} (σ : gmap loc X) : block :=
   let loclst : list loc := elements (dom _ σ : gset loc) in
   let blockset : gset block := foldr (λ l, ({[loc_chunk l]} ∪.)) ∅ loclst in
